\documentclass[dvipdfmx]{jsarticle}
\usepackage[english]{babel}
\usepackage{amsmath}
\begin{document}

\title{Homework3}
\author{}
\maketitle

\section{My Information}
Student number:
//
faculty of commerce 4th
ho-class
\section{Deriviation of Probability of MultinominalLogitModel}

If the reduals $\epsilon$ are independently and identically distributed with the type I extreme-value distribution whose comulative distribution function (CDF) is
\begin{equation}
  F(\epsilon_i - \epsilon) = exp(-e^{-\epsilon})
\end{equation}

and whose probability density function (PDF) is

\begin{equation}
  f(\epsilon) = exp(-\epsilon - e^{-\epsilon_i})
\end{equation}

then we can show that

\begin{equation}
  Prob(Y_i = 1 | X) = \frac{e^V_i}{\sum_{j=1}^{m}e^V_j}
\end{equation}

The condition $Y^*=Max(Y^*_1, Y^*_2, Y^*_3..., Y^*_m)$
implies

\begin{equation}
 \epsilon_i + V_i > \epsilon_j + V_j　\  for \ all \ j \neq i
\end{equation}

or

\begin{equation}
 \epsilon_i <  \epsilon_j + V_j - V_i  \  for \  all \  j \neq i
\end{equation}

Hence , if $\epsilon_1, \epsilon_2, ... \epsilon_m $ are identically and independently distributed , with CDF given by 1,then


\begin{equation}
  Prob(Y_i = 1) = Prob(\epsilon_i <  \epsilon_j + V_j - V_i ) \  for \  all \  j \neq i
 \end{equation}

 \begin{equation}
   = \int _{-\infty}^\infty\prod_{j\neq i} F(\epsilon_i + V_i - V_j)*f(\epsilon_i)d\epsilon_i
 \end{equation}

 where $F(・)$and$f(・)$are given by (1), (2) respectively. Now

 \begin{equation}
 \prod_{j\neq i}F(\epsilon_i + V_i - V_j)f(\epsilon_i) = \prod{j \neq i}exp(-e^{-\epsilon_i} - V_i + V_j)exp(-\epsilon_i - e^{-\epsilon_i})
\end{equation}

\begin{equation}
  = exp[\epsilon_i - e^{-\epsilon_i}(1 + \sum_{j \neq i}\frac{e^{V_j}}{e^{V_i}})]
 \end{equation}


 If we write (7) as

 \begin{equation}
  = \lambda_i = log(1 + \sum_{j \neq i}\frac{e^{V_j}}{e^{V_i}})
 \end{equation}

 We can write (7) as
 \begin{equation}
  \int _{-\infty}^\infty exp(-\epsilon^*_i-e^{-(\epsilon_i - \lambda_i)})d\epsilon_i
 \end{equation}
 \begin{equation}
  = exp(-\lambda_i)\int_{-\infty}^{\infty}exp(-\epsilon^*_i-e^{-e^*_i})d\epsilon_i \  where \  -e^*_j =  \epsilon_i - \lambda
 \end{equation}
 \begin{equation}
  = exp(\lambda_i)
 \end{equation}
 \begin{equation}
  = \frac{e^{V_i}}{\sum_{j = 1}^m e^{V_j}}
 \end{equation}
\section{Summary}

I don't know differentiate of fractional function, I learned it.

I'm getting used to latex
\end{document}
